Barasz.lean
@@ -1,6 +1,5 @@
 import Barasz.GL
-import Barasz.Agent
+import Barasz.ModalAgent
 import Barasz.FixedPoint
 import Barasz.Cooperation
-import Barasz.Game
-import Barasz.Equilibrium
+import Barasz.Behavioral
